pcuic/theories/Conversion/PCUICOnFreeVarsConv.v
@@ -1,0 +1,133 @@
+(* Distributed under the terms of the MIT license. *)
+From Coq Require Import Morphisms. 
+From MetaCoq.Template Require Import config utils.
+From MetaCoq.PCUIC Require Import PCUICAst PCUICAstUtils PCUICCases PCUICInduction
+     PCUICLiftSubst PCUICUnivSubst PCUICContextRelation PCUICSigmaCalculus PCUICClosed 
+     PCUICOnFreeVars PCUICTyping PCUICReduction PCUICGlobalEnv PCUICWeakeningEnvConv PCUICClosedConv
+     PCUICWeakeningEnvTyp PCUICInstDef PCUICRenameDef PCUICRenameConv.
+
+Require Import ssreflect ssrbool.
+From Equations Require Import Equations.
+
+Lemma on_free_vars_rename P f t :
+  on_free_vars P (rename f t) = on_free_vars (P ∘ f) t.
+Admitted. 
+
+Lemma rename_on_free_vars n t f :
+  on_free_vars (shiftnP n xpred0) t -> rename (shiftn n f) t = t.
+Admitted.
+
+
+Lemma urename_on_free_vars_shift P Γ Δ f u (Ξ:list context_decl) : 
+   let sP := shiftnP #|Γ| P in
+   urenaming sP Δ Γ f -> 
+   is_closed_context Γ -> 
+   is_closed_context Δ -> 
+   on_free_vars (shiftnP #|Ξ| (shiftnP #|Γ| xpred0)) u -> 
+   on_free_vars (shiftnP #|Ξ| (shiftnP #|Δ| xpred0)) 
+                (rename (shiftn #|Ξ| f) u).
+   intros sP hf HΓ HΔ Hu. rewrite on_free_vars_rename.
+   eapply on_free_vars_impl. 2: tea. clear Hu. intros n Hn.
+   apply urenaming_context with (Ξ:=Ξ) in hf. 
+   unfold urenaming in hf. 
+   specialize (hf n). destruct (nth_error (Γ,,, Ξ) n) eqn : Hnth.
+   - specialize (hf c); cbn in hf. forward hf. 
+     * unfold shiftnP in Hn. unfold sP , shiftnP.
+       toProp. toProp Hn. destruct Hn.
+       + intuition.
+       + right. toProp. toProp H. destruct H; intuition.       
+     * destruct (hf eq_refl) as [decl' [Hfn _]].
+       clear hf Hn. unfold sP , shiftnP. rewrite orb_false_r. 
+       assert (shiftn #|Ξ| f n < #|Δ,,, rename_context f Ξ|). 
+       { eapply nth_error_Some'. exists decl'. eauto. }
+       rewrite app_context_length in H.
+       rewrite rename_context_length in H.
+       toProp. clear -H.
+       repeat rewrite PeanoNat.Nat.ltb_lt. lia. 
+  - rewrite nth_error_None in Hnth. rewrite app_context_length in Hnth. unfold shiftnP in *. toProp Hn. toProp. unfold shiftn.
+    clear -Hn Hnth. destruct Hn.
+    * toProp H. intuition.
+    * toProp H. destruct H; [toProp H |]; intuition.      
+Defined.  
+
+Lemma urename_is_open_term P Γ Δ f u : let sP := shiftnP #|Γ| P in
+   urenaming sP Δ Γ f -> is_closed_context Γ -> is_closed_context Δ -> is_open_term Γ u -> is_open_term Δ (rename f u).
+Proof.
+  intros sP hf HΓ HΔ Hu.
+  unfold is_open_term.
+  rewrite <- (shiftnP0 (shiftnP #|Δ| xpred0)).
+  rewrite <- (shiftn0 f).
+  eapply urename_on_free_vars_shift with (Ξ:=[]); eauto.
+  rewrite shiftnP0; eauto. 
+Defined. 
+
+
+
+
+Lemma on_free_vars_ctx_inst_case_context 
+  P (Γ : list context_decl) (pars : list term)
+  (puinst : Instance.t) (pctx : list context_decl) :
+  forallb (on_free_vars (shiftnP #|Γ| P)) pars ->
+  on_free_vars_ctx (closedP #|pars| xpredT) pctx ->
+  on_free_vars_ctx P Γ ->
+  on_free_vars_ctx P (Γ,,, inst_case_context pars puinst pctx).
+Proof.
+  intros. rewrite on_free_vars_ctx_app H1 /=.
+  eapply on_free_vars_ctx_inst_case_context; trea; solve_all.
+  rewrite test_context_k_closed_on_free_vars_ctx //.
+Qed.
+
+
+Lemma rename_context_on_free_vars f n l  :
+on_free_vars_ctx (closedP n xpredT) l ->  
+rename_context (shiftn n f) l = l.
+Proof.
+  intro Hclosed. 
+  unfold on_free_vars_ctx in Hclosed. 
+  unfold rename_context, fold_context_k. 
+  induction l; eauto.
+  cbn in *. rewrite alli_app in Hclosed. toProp Hclosed.
+  destruct Hclosed as [H Hclosed]. 
+  rewrite mapi_rec_app. rewrite List.distr_rev.
+  rewrite IHl; eauto.
+  cbn in *. f_equal.
+  toProp Hclosed. destruct Hclosed as [Hclosed _].
+  destruct a; unfold map_decl; cbn.
+  unfold on_free_vars_decl in Hclosed. 
+  unfold test_decl in Hclosed.
+  toProp Hclosed. cbn in Hclosed.
+  destruct Hclosed as [Hbody Htype].
+  f_equal.
+  - destruct decl_body; eauto; cbn in *. 
+    f_equal. rewrite closedP_shiftnP in Hbody.
+    rewrite shiftnP_add in Hbody. rewrite shiftn_add.
+    apply rename_on_free_vars; eauto.
+  - rewrite closedP_shiftnP in Htype.
+    rewrite shiftnP_add in Htype. rewrite shiftn_add.
+    apply rename_on_free_vars; eauto.
+Defined. 
+
+Lemma inst_case_predicate_context_rename f p :  
+  on_free_vars_ctx (closedP #|pparams p| xpredT) (pcontext p) ->
+  inst_case_predicate_context (rename_predicate f p) = rename_context f (inst_case_predicate_context p).
+Proof. 
+  intro Hclosed. unfold inst_case_predicate_context.
+  unfold pparams at 1. cbn.
+  replace (pcontext p) with 
+  (rename_context (shiftn #|(pparams p)| f) (pcontext p)) at 1.
+  - rewrite <- rename_inst_case_context. reflexivity.
+  - apply rename_context_on_free_vars; eauto.
+Defined.   
+
+Lemma inst_case_branch_context_rename f p x :
+on_free_vars_ctx (closedP #|pparams p| xpredT) (bcontext x) ->  
+inst_case_branch_context (rename_predicate f p) 
+     (rename_branch f x) =
+     rename_context f (inst_case_branch_context p x).
+Proof.
+  intro Hclosed. unfold inst_case_branch_context. cbn. 
+  replace (bcontext x) with 
+  (rename_context (shiftn #|(pparams p)| f) (bcontext x)) at 1.
+  - rewrite <- rename_inst_case_context. reflexivity.
+  - apply rename_context_on_free_vars; eauto.
+Defined.     
